Redefine paths for better inductive structure

AttarchTrans.v
@@ -2,13 +2,24 @@ Require Import Ctl.Definition.
 Require Import TransitionSystems.
 Require Import Privilege.
 
-(* Maybe sel4 should not be its own place *)
 Inductive component : Set := 
-  | sel4 
   | platam 
   | vmm 
   | useram
   | malicious_linux_component.
+
+Inductive boot_ev_t :=
+  | good_boot_ev 
+  | bad_boot_ev.
+Inductive vm_ev_t :=
+  | good_vm_ev
+  | bad_vm_ev.
+Inductive platam_key_t :=
+  | good_platam_key
+  | bad_platam_key.
+Inductive useram_key_t :=
+  | good_useram_key
+  | bad_useram_key.
 
 Record mem_store v : Type := mkMem_store 
   { acc_at: access component
@@ -18,31 +29,38 @@ Arguments acc_at {v}%type_scope.
 Arguments val_at {v}%type_scope.
 
 Record attarch_global := mkAttarchGl
-  { boot_ev    : mem_store nat
-  ; vm_ev      : mem_store nat
-  ; useram_key : mem_store nat
+  { boot_ev    : mem_store boot_ev_t
+  ; vm_ev      : mem_store vm_ev_t
+  ; platam_key : mem_store platam_key_t
+  ; useram_key : mem_store useram_key_t
   }.
 
-Definition set_boot_ev (st: attarch_global) (m: mem_store nat) : attarch_global :=
+Definition set_boot_ev (st: attarch_global) m : attarch_global :=
   {| boot_ev    := m; 
      vm_ev      := vm_ev st;
+     platam_key := platam_key st;
      useram_key := useram_key st |}.
-Definition set_vm_ev (st: attarch_global) (m: mem_store nat) : attarch_global :=
+Definition set_vm_ev (st: attarch_global) m : attarch_global :=
   {| boot_ev    := boot_ev st;
      vm_ev      := m;
+     platam_key := platam_key st;
      useram_key := useram_key st |}.
-Definition set_useram_key (st: attarch_global) (m: mem_store nat) : attarch_global :=
+Definition set_useram_key (st: attarch_global) m : attarch_global :=
   {| boot_ev    := boot_ev st; 
      vm_ev      := vm_ev st;
+     platam_key := platam_key st;
      useram_key := m |}.
+Definition set_platam_key (st: attarch_global) m : attarch_global :=
+  {| boot_ev    := boot_ev st; 
+     vm_ev      := vm_ev st;
+     platam_key := m;
+     useram_key := useram_key st |}.
 
-Definition good_boot_ev : nat.
-exact 0. Qed.
-Definition bad_boot_ev  : nat.
-exact 0. Qed.
+
 Definition initial_global_state_good :=
-  {| boot_ev    := {|acc_at := allAcc; val_at := Some good_boot_ev|};
+  {| boot_ev    := {|acc_at := readonly; val_at := Some good_boot_ev|};
      vm_ev      := {|acc_at := allAcc; val_at := None|};
+     platam_key := {|acc_at := allAcc; val_at := None|};
      useram_key := {|acc_at := allAcc; val_at := None|}
   |}.
 
@@ -61,34 +79,42 @@ Inductive useram_trans : transition attarch_global useram_state :=
       acc_at (useram_key st) useram read ->
       useram_trans 
         (st, useram_waiting_key)
-        (st, useram_waiting_request)
- (* | useram_get_request : useram_trans 
-      (s, useram_waiting_key)
-      (s,useram_) *)
-  .
-(* Definition useram_strans := stransition useram_trans. *)
+        (st, useram_waiting_request).
 
 Inductive platam_state : Set :=
   | platam_init
+  | platam_measure
   | platam_appraise
   | platam_run.
 
-Definition good_vm_ev : nat. Admitted.
-Definition bad_vm_ev  : nat. Admitted.
-Definition good_useram_key : nat. Admitted.
+
 Inductive useram_key_acc : access component :=
   | useram_useram_key_read  : useram_key_acc useram read
   | platam_useram_key_read  : useram_key_acc platam read
   | platam_useram_key_write : useram_key_acc platam write.
 
+Definition acquire_key boot_ev :=
+  match boot_ev with 
+  | good_boot_ev => good_platam_key
+  | bad_boot_ev => bad_platam_key
+  end.
+
 Inductive platam_trans : transition attarch_global platam_state :=
+  | platam_acquire_key : forall st boot_ev_val,
+      acc_at (boot_ev st) platam read ->
+      val_at (boot_ev st) = Some boot_ev_val ->
+      platam_trans 
+        (st, platam_init)
+        (set_platam_key st 
+          {|acc_at := private platam; val_at := Some (acquire_key boot_ev_val)|}, 
+          platam_measure)
   | platam_measure_good_vm : forall st,
       platam_trans
-        (st, platam_init)
+        (st, platam_measure)
         (set_vm_ev st {|acc_at := private platam; val_at := Some good_vm_ev|}, platam_appraise)
   | platam_measure_bad_vm : forall st,
       platam_trans
-        (st, platam_init)
+        (st, platam_measure)
         (set_vm_ev st {|acc_at := private platam; val_at := Some bad_vm_ev|}, platam_appraise)
   | platam_release_key : forall st,
       acc_at (vm_ev st) platam read ->
@@ -117,16 +143,15 @@ Inductive attarch_state : Set :=
   | sel4_run : platam_state * vm_state -> attarch_state.
 
 Inductive attarch_trans : transition attarch_global attarch_state :=
-  (* | good_boot : forall st,
-      (fst (boot_ev st)) sel4 read ->
-      (snd (boot_ev st)) = good_boot_ev ->
-      attarch_trans 
-        (st, boot_from_good_plat)
-        (st, sel4_run (platam_init, vm_init)) *)
-  | attarch_boot : forall st,
+  (* TODO: add some boolean "good seL4 image" field to global state to determine boot? *)
+  | good_boot : forall st,
       attarch_trans 
         (st, boot)
-        (st, sel4_run (platam_init, vm_init))
+        (set_boot_ev st {|acc_at := readonly; val_at := Some good_boot_ev|}, sel4_run (platam_init, vm_init))
+  | bad_boot : forall st,
+      attarch_trans 
+        (st, boot)
+        (set_boot_ev st {|acc_at := readonly; val_at := Some bad_boot_ev|}, sel4_run (platam_init, vm_init))
   | component_step : forall g g' s s',
       (platam_trans ⊔ vm_trans) (g,s) (g',s') ->
       attarch_trans 
