Ctl/Paths.v
@@ -4,29 +4,219 @@ Require Import BinaryRelations.
 Require Import Coq.Relations.Relation_Definitions.
 Require Import Coq.Relations.Relation_Operators.
 
-Inductive path {state} (R: relation state) : state -> nat -> Type := 
+(* Old path defn *)
+(* Inductive path {state} (R: relation state) : state -> nat -> Prop := 
   | path_trivial : forall s, path R s 0
   | path_step : forall s s' n,
       R s s' ->
       path R s' n ->
       path R s (S n).
 Arguments path_trivial {state R}%type_scope.
-Arguments path_step    {state R}%type_scope.
+Arguments path_step    {state R}%type_scope. *)
 
-Inductive in_path {state} {R: relation state} {s}
-  : state -> forall {n}, path R s n -> Prop :=
-  | in_path_head_trivial :
-      in_path s (path_trivial s)
-  | in_path_head_step : forall s' n r p,
-      in_path s (path_step s s' n r p)
-  | in_path_tail : forall s' x n r p,
-      @in_path state R s' x n p ->
-      in_path x (path_step s s' n r p).
+(* A length-indexed transition sequence
+   Essentially a reflexive-transitive closure, where the sequence of steps is 
+   transparent (plus the type-level length info).
+*)
+Inductive path_to {state} (R: relation state): nat -> state -> state -> Prop :=
+  | path_to_refl : forall s,
+      path_to R 0 s s
+  | path_to_step : forall s x x' n,
+      R x x' ->
+      path_to R n s x ->
+      path_to R (S n) s x'.
+Arguments path_to_refl {state R}%type_scope.
+Arguments path_to_step {state R}%type_scope.
+
+(* (almost) transitivity *)
+Definition path_to_combine {state n m} {R: relation state} {x y z}:
+  path_to R n x y ->
+  path_to R m y z ->
+  path_to R (n+m) x z.
+intros path_xy path_yz; revert n x path_xy.
+induction path_yz; intros.
++ rewrite PeanoNat.Nat.add_0_r. 
+  assumption.
++ rewrite PeanoNat.Nat.add_succ_r.
+  eapply path_to_step.
+  * eassumption.
+  * applyc IHpath_yz.
+    assumption.
+Defined.
+
+Definition path {state} (R: relation state) (n: nat) (s: state) :=
+  exists s', path_to R n s s'.
+
+Theorem path_refl {state}: forall (R: relation state) s,
+  path R 0 s.
+Proof using.
+  intros.
+  econstructor.
+  constructor.
+Qed.
+
+Theorem path_step {state}: forall (R: relation state) n s x x',
+  R x x' ->
+  path_to R n s x ->
+  path R (S n) s.
+Proof using.
+  intros.
+  econstructor.
+  econstructor; eassumption.
+Qed.
+
+Definition path_from_path_to {state} {R: relation state} {n s s'}
+  (p: path_to R n s s') : path R n s :=
+  ex_intro _ s' p.
+
+Inductive in_path_to_at {state} {R: relation state} {s}
+  : forall {s'}, state -> nat -> forall {n}, path_to R n s s' -> Prop :=
+  | in_path_to_at_head_refl :
+      in_path_to_at s 0 (path_to_refl s)
+  | in_path_to_at_head_step : forall x x' n r p,
+      in_path_to_at x' n (path_to_step s x x' n r p)
+  | in_path_to_at_tail : forall x x' y n m r p,
+      in_path_to_at y m p ->
+      in_path_to_at y m (path_to_step s x x' n r p).
+
+Inductive in_path_at {state} {R: relation state} {n s} 
+  : state -> nat -> path R n s -> Prop :=
+  | in_path_at_rule : forall x m s' (p: path_to R n s s'),
+      in_path_to_at x m p ->
+      in_path_at x m (path_from_path_to p).
+
+Inductive in_path_to {state} {R: relation state} {s}
+  : forall {s'}, state -> forall {n}, path_to R n s s' -> Prop :=
+  | in_path_to_head_refl :
+      in_path_to s (path_to_refl s)
+  | in_path_to_head_step : forall x x' n r p,
+      in_path_to x' (path_to_step s x x' n r p)
+  | in_path_to_tail : forall x x' y n r p,
+      in_path_to y p ->
+      in_path_to y (path_to_step s x x' n r p).
+
+Inductive in_path {state} {R: relation state} {n s} 
+  : state -> path R n s -> Prop :=
+  | in_path_rule : forall x s' (p: path_to R n s s'),
+      in_path_to x p ->
+      in_path x (path_from_path_to p).
+
+Theorem in_path_from_in_path_to {state}:
+  forall (R: relation state) n s s' (p: path_to R n s s') x,
+    in_path_to x p ->
+    in_path x (path_from_path_to p).
+Proof using.
+  intros.
+  destruct H; repeat constructor.
+  assumption.
+Qed. 
+
+Theorem in_path_at_from_in_path_to_at {state}:
+  forall (R: relation state) n s s' i (p: path_to R n s s') x,
+    in_path_to_at x i p ->
+    in_path_at x i (path_from_path_to p).
+Proof using.
+  intros.
+  destruct H; repeat constructor.
+  assumption.
+Qed. 
+
+Theorem in_path_to_impl_in_path_to_at {state} {R: relation state} {n s s'}:
+  forall x (p: path_to R n s s'), 
+    in_path_to x p ->
+    exists i, in_path_to_at x i p.
+Proof.
+  intros x p H.
+  induction H. 
+  - eexists; constructor.
+  - eexists; constructor.
+  - destruct exists IHin_path_to i.
+    eexists.
+    constructor.
+    eassumption.
+Qed.
+
+Theorem in_path_to_at_impl_in_path_to {state} {R: relation state} {n s s'}:
+  forall x i (p: path_to R n s s'),
+    in_path_to_at x i p ->
+    in_path_to x p.
+Proof.
+  intros x i p H.
+  induction H; constructor.
+  assumption.
+Qed.
+
+Theorem in_path_impl_in_path_at {state} {R: relation state} {n s}:
+  forall x (p: path R n s), 
+    in_path x p ->
+    exists i, in_path_at x i p.
+Proof.
+  intros x p H.
+  invc H.
+  apply in_path_to_impl_in_path_to_at in H0.
+  destruct exists H0 i.
+  exists i.
+  constructor.
+  assumption.
+Qed.
+
+Theorem in_path_at_impl_in_path {state} {R: relation state} {n s}:
+  forall x i (p: path R n s),
+    in_path_at x i p ->
+    in_path x p.
+Proof.
+  intros x i p H.
+  invc H.
+  constructor.
+  eapply in_path_to_at_impl_in_path_to.
+  eassumption.
+Qed.
+
+Definition in_path_to_before {state} {R: relation state} {n s s'}
+  x i (p: path_to R n s s') := 
+  exists j, j < i /\ in_path_to_at x i p.
+
+Definition in_path_before {state} {R: relation state} {n s} x i (p: path R n s) := 
+  exists j, j < i /\ in_path_at x i p.
+
 
 (* A single-step path *)
-Definition path_singleton {state} {R: relation state} {x y} (r: R x y) : path R x 1 :=
-  path_step x y 0 r (path_trivial y).
+Definition path_to_singleton {state} {R: relation state} {x y} (r: R x y)
+  : path_to R 1 x y :=
+  path_to_step x x y 0 r (path_to_refl x).
 
+Definition path_singleton {state} {R: relation state} {x y} (r: R x y)
+  : path R 1 x :=
+  path_from_path_to (path_to_singleton r).
+
+
+Theorem path_to_step_rev {state}: forall (R: relation state) n s s' x,
+  R s s' ->
+  path_to R n s' x ->
+  path_to R (S n) s x.
+Proof using.
+  intros R n s s' x Hstep Hpath.
+  induction Hpath.
+  - apply path_to_singleton.
+    assumption.
+  - econstructor.
+    + eassumption.
+    + applyc IHHpath.
+      assumption.
+Qed.
+
+Theorem path_step_rev {state}: forall (R: relation state) n s s',
+  R s s' ->
+  path R n s' ->
+  path R (S n) s.
+Proof using.
+  intros R n s s' Hstep Hpath.
+  destruct exists Hpath x.
+  eapply path_from_path_to.
+  eapply path_to_step_rev; eassumption.
+Qed.
+
+(*
 Require Import Psatz.
 Definition path_pop n {state} {R: relation state} {m s} (p: path R s m) 
   : {s' & path R s' (m-n)}.
@@ -106,23 +296,28 @@ induction n.
       apply sfw.
       eapply rtc_alt_trans; eassumption.
 Defined.
+*)
 
-Definition path_combineT {state} {R: relation state}: 
-  forall s x x' n n' (p: path R s n) (p': path R x n'),
-  in_path x p -> in_path x' p' -> 
-  {n'' & {p'': path R s n'' & in_path x' p''}}.
-  (* n' <= n'' <= n+n' *)
-intros s x x' n n' p p' Hx Hx'.
-try induction Hx.
-(* Might not be definable, since it depends on value of Prop Hx *)
-Abort.
-
-Theorem path_combine {state} {R: relation state}: 
-  forall s x x' n n' (p: path R s n) (p': path R x n'),
-  in_path x p -> in_path x' p' -> 
-  exists n'' (p'': path R s n''), in_path x' p''.
+(*
+Theorem in_path_at_combine {state} {R: relation state}: 
+  forall n m i j x x' y y' s (p: path n R x x') (p': path m R y y'),
+    in_path_at y i p -> 
+    in_path_at s j p' -> 
+    (* Could also be path size (i+j) if we wanted to cut it as short as possible *)
+    (* exists p'': path (i+m) R x y', in_path_at s (i+j) p''. *)
+    exists l (p'': path l R x y'), in_path_at s (i+j) p''.
 Proof.
-  intros s x x' n n' p p' Hx Hx'.
+  intros n m i j x x' y y' s p p' Hy Hs.
+  revert m j y' s p' Hs.
+  induction Hy; intros; try solve [eauto].
+  eapply path_step in p; [|eassumption]; clear r.
+  exists (S n + m) (path_combine p p').
+  induction Hs.
+  - simpl.
+  
+  (* Check (path_combine (path_step _ _ _ _ r p) p'). *)
+
+  (* intros s x i x' j n n' p p' Hx Hx'.
   induction Hx; [eauto|eauto|].
   specialize (IHHx p' Hx').
   destruct exists IHHx n'' p''.
@@ -130,28 +325,130 @@ Proof.
   exists (path_step s s' n'' r p'').
   constructor.
   assumption.
+Qed. *)
+Admitted.
+*)
+
+(* 
+Theorem in_path_at_combine {state} {R: relation state}: 
+  forall s x i x' j n n' (p: path R s n) (p': path R x n'),
+    in_path_at x i p -> in_path_at x' j p' -> 
+    exists n'' (p'': path R s n''), in_path_at x' (i+j) p''.
+Proof.
+  intros s x i x' j n n' p p' Hx Hx'.
+  induction Hx; [eauto|eauto|].
+  specialize (IHHx p' Hx').
+  destruct exists IHHx n'' p''.
+  exists (S n'').
+  exists (path_step s s' n'' r p'').
+  constructor.
+  assumption.
+Qed. *)
+
+(* Theorem in_path_combine {state} {R: relation state}: 
+  forall s x x' n n' (p: path R s n) (p': path R x n'),
+    in_path x p -> in_path x' p' -> 
+    exists n'' (p'': path R s n''), in_path x' p''.
+Proof.
+  intros.
+  apply in_path_eq_in_path_at in H, H0.
+  destruct exists H i.
+  destruct exists H0 j.
+  eapply in_path_at_combine in H0; [|eassumption].
+  destruct exists H0 n'' p''.
+  exists n'' p''.
+  eapply in_path_at_to_in_path.
+  eassumption.
+Qed.  *)
+
+Theorem path_to_impl_rtc {state}: forall (R: relation state) n s s',
+  path_to R n s s' -> R^* s s'.
+Proof.
+  intros R n s s' H.
+  induction H.
+  - reflexivity.
+  - econstructor; eassumption.
 Qed.
   
-Theorem path_to_rtc {state}: forall (R: relation state) s s' n (p: path R s n),
-  in_path s' p -> R^* s s'.
+Theorem in_path_impl_rtc {state}:
+  forall (R: relation state) n s s' (p: path R n s),
+    in_path s' p -> R^* s s'.
 Proof.
-  intros R s s' n p Hin.
-  induction Hin.
+  intros R n s s' p Hin.
+  invc Hin.
+  induction H.
   - constructor.
-  - constructor.
-  - eapply rtc_alt_trans; eassumption.
+  - econstructor.
+    + eassumption.
+    + eapply path_to_impl_rtc.
+      eassumption.
+  - assumption.
 Qed.
 
-Lemma rtc_to_path {state}: forall (R: relation state) s s',
-  R^* s s' -> exists n (p: path R s n), in_path s' p.
-Proof.
-  intros R s s' Hsteps.
-  apply rtc_1n_n1_equiv in Hsteps.
-  induction Hsteps.
-  - repeat eexists. econstructor.
-  - destruct exists IHHsteps n p;
+Lemma rtc_impl_path_to {state}: forall (R: relation state) s s',
+  R^* s s' -> exists n, path_to R n s s'.
+Proof using.
+  intros R s s' H.
+  induction H.
+  - eexists. apply path_to_refl.
+  - destruct exists IHclos_refl_trans_n1 n.
     exists (S n).
-    exists (path_step _ _ _ H p).
-    constructor.
-    assumption.
+    econstructor; eassumption.
+Qed.
+
+(*
+(* Print clos_refl_trans_n1. *)
+Inductive rtc_len {A} {R: relation A} : nat -> R^* x y -> Prop :=
+  | rtc_len_0 : 
+      rtc_len 0 
+*)
+Inductive in_rtc {state} {R: relation state} {s}
+  : forall {s'}, state -> R^* s s' -> Prop :=
+  | in_rtc_head_refl :
+      in_rtc s (rtn1_refl state R s)
+  | in_rtc_head_step : forall x x' r p,
+      in_rtc x' (rtn1_trans state R s x x' r p)
+  | in_rtc_tail : forall x x' y r p,
+      in_rtc y p ->
+      in_rtc y (rtn1_trans state R s x x' r p)
+  .
+
+Theorem foo {state}: forall (R: relation state) n s s' (p: path_to R n s s') x,
+  in_path_to x p ->
+  in_rtc x (path_to_impl_rtc _ _ _ _ p).
+
+Theorem in_path_to_first {state}:
+  forall (R: relation state) n s s' (p: path_to R n s s'),
+    in_path_to s p.
+Proof using.
+  intros.
+  elim p.
+  induction p.
+Admitted.
+
+Theorem in_path_to_last {state}:
+  forall n (R: relation state) s s' (p: path_to n R s s'),
+    in_path_to s' p.
+Proof using.
+  intros.
+  destruct p; constructor.
+Qed.
+
+Theorem in_path_last {state}:
+  forall n (R: relation state) s s' (p: path_to n R s s'),
+    in_path s' (path_from_path_to p).
+Proof using.
+  intros.
+  eapply in_path_from_in_path_to.
+  apply in_path_to_last.
+Qed.
+
+Lemma rtc_impl_in_some_path {state}: forall (R: relation state) s s',
+  R^* s s' -> exists n (p: path n R s), in_path s' p.
+Proof.
+  intros R s s' H.
+  apply rtc_impl_path_to in H.
+  destruct exists H n.
+  exists n.
+  exists (path_from_path_to H).
 Qed.
