Ctl/Definition.v
@@ -44,8 +44,13 @@ Notation "P ∨ Q" := (TDisj P Q) (at level 55, right associativity).
 Notation "P --> Q" := (TImpl P Q) (at level 68,  right associativity).
 Notation "P <--> Q" := ((P --> Q) ∧ (Q --> P)) (at level 65,  right associativity).
 Notation "¬ P" := (TNot P) (at level 40).
-Notation "'A' [ P 'U' Q ]" := (AU P Q) (at level 40).
-Notation "'E' [ P 'U' Q ]" := (EU P Q) (at level 40).
+Notation "'A' [ P 'U' Q ]" := (AU P Q) (at level 40, format "'A' [ P  'U'  Q ]").
+Notation "'E' [ P 'U' Q ]" := (EU P Q) (at level 40, format "'E' [ P  'U'  Q ]").
+
+(* Add "W" operator?
+   "Weak" until, AKA the "unless" operator. Like the until operator, but the
+   second condition does not ever have to come true.
+ *)
 
 Reserved Notation "M @ s ⊨ P" (at level 70, format "M  @ s  ⊨  P").
 Reserved Notation "M @ s ⊭ P" (at level 70, format "M  @ s  ⊭  P").
@@ -61,12 +66,18 @@ Fixpoint tEntails {state} (R: relation state) (s: state) (tp: TProp state) : Pro
   | P --> Q => R @s ⊨ P -> R @s ⊨ Q
   | AX P => forall s', R s s' -> R @s' ⊨ P
   | EX P => exists s', R s s' -> R @s' ⊨ P
-  | AG P => forall n, forall (p: path R s n), forall s', in_path s' p -> R @s' ⊨ P
-  | EG P => forall n, exists (p: path R s n), forall s', in_path s' p -> R @s' ⊨ P
-  | AF P => exists n, forall (p: path R s n), exists s', in_path s' p /\ R @s' ⊨ P
-  | EF P => exists n, exists (p: path R s n), exists s', in_path s' p /\ R @s' ⊨ P
-  (* TODO: AU and EU *)
-  | _ => False
+  | AG P => forall n, forall p: path R s n, forall s', in_path s' p -> R @s' ⊨ P
+  | EG P => forall n, exists p: path R s n, forall s', in_path s' p -> R @s' ⊨ P
+  | AF P => exists n, forall p: path R s n, exists s', in_path s' p /\ R @s' ⊨ P
+  | EF P => exists n, exists p: path R s n, exists s', in_path s' p /\ R @s' ⊨ P
+  | A[P U Q] => forall n, forall p: path R s n,
+      exists sQ i, in_path_at sQ i p /\ 
+        R @sQ ⊨ Q /\
+        forall sP, in_path_before sP i p -> R @sP ⊨ P
+  | E[P U Q] => forall n, exists p: path R s n,
+      exists sQ i, in_path_at sQ i p /\ 
+        R @sQ ⊨ Q /\
+        forall sP, in_path_before sP i p -> R @sP ⊨ P
   end
   where "M @ s ⊨ P" := (tEntails M s P)
     and "M @ s ⊭ P" := (~ M @s ⊨ P).
